Upd

Opcodes.fst
@@ -2,6 +2,8 @@ module Opcodes
 
 open StackBC
 open FStar.Seq
+open Prims 
+open SeqExtension
 
 module Stack = StackBC
 module Seq = FStar.Seq
@@ -53,7 +55,9 @@ let op_hash160 st_before line_before result_before =
 (*val split: #a:Type -> s:seq a -> i:nat{(0 <= i /\ i <= length s)} -> Tot (seq a * seq a) *)
 val op_push : st_before: stackBC (seq nat){ capacity st_before > 0}
 				-> line_before : seq nat {Seq.length line_before > 0 /\ 
-											Seq.length line_before > 1 + (Seq.head line_before)} ->
+											Seq.length line_before > 1 + (Seq.head line_before) /\
+											((Seq.head line_before > 0) && (Seq.head line_before < 76))
+											} ->
 				result_before: bool{result_before = true}
 				-> Tot(st: stackBC (seq nat) {Stack.length st > 0 /\ 
 		Seq.length (Stack.index st 0) = Seq.head line_before} *  
@@ -69,3 +73,189 @@ let op_push st_before line_before result_before =
 		let element = fst line in 
 		let stack_push1 = Stack.push st_before element  in 
 		(stack_push1, snd line, result_before)
+
+val op_equalverify: st_before : stackBC (seq nat){Stack.length st_before > 1} -> 
+			line_before : seq nat {Seq.length line_before > 0 /\ Seq.head line_before = 136} ->
+			result_before : bool{result_before = true} -> 
+			Tot(st: stackBC (seq nat) {Stack.length st_before >= 0} * 
+			line : seq nat{Seq.length line = Seq.length line_before -1} * result: bool)
+
+let op_equalverify st_before line_before result_before = 
+	let pop = Stack.pop st_before in 
+	let elem1 = fst pop in 
+	let pop2 = Stack.pop (snd pop) in 
+	let elem2 = fst pop2 in 
+	let result = (elem1 = elem2) in 
+	let line = Seq.tail line_before in  
+	(snd pop2, line, result)
+
+val op_false: st_before: stackBC (seq nat) {Stack.capacity st_before > 0}-> 
+				line_before : seq nat {Seq.length line_before > 0 /\ Seq.head line_before = 0}-> 
+				result_before : bool{result_before = true} ->
+				Tot(st: stackBC (seq nat){Stack.length st = Stack.length st_before + 1} * 
+				line : seq nat {Seq.length line = Seq.length line_before -1} * result: bool)
+
+let op_false st_before line_before result_before = 
+	let element = Seq.createEmpty  in 
+	let stack_push1 = Stack.push st_before element in 
+	let line = Seq.tail line_before in 
+	(stack_push1, line, result_before)
+
+val get_bytes_push: number: nat{number = 1 || number = 2 || number = 4} ->  
+					line_before : seq nat{Seq.length line_before > number} -> 
+					Tot (nat * line: seq nat{Seq.length line = Seq.length line_before - number})
+let get_bytes_push number line_before = 
+	(*  I dont wanna have a recursion call while the standart is given only 1/2/4*)
+	let r = 0 in
+	if (number  = 1 ) then 
+		let r = Seq.head line_before in (r, Seq.tail line_before)
+	else if (number = 2) then 
+		let r = Seq.head line_before in 
+		let line_temp = Seq.tail line_before in 
+		let r = op_Multiply r 256 + (Seq.head line_temp) in 
+		let line_temp = Seq.tail line_temp in (r, line_temp)
+	else 
+		let r = Seq.head line_before in 
+		let line_temp = Seq.tail line_before in 
+		let r = op_Multiply r 256  + Seq.head line_temp in 
+		let line_temp = Seq.tail line_temp in 
+		let r = op_Multiply r 256  + Seq.head line_temp in 
+		let line_temp = Seq.tail line_temp in 
+		let r = op_Multiply r 256  + Seq.head line_temp in 
+		let line_temp = Seq.tail line_temp in (r, line_temp)
+
+val op_push1: st_before : stackBC (seq nat) {Stack.capacity st_before > 0} ->
+				line_before : seq nat {
+					Seq.length line_before > 0 /\ Seq.head line_before = 76 /\ 
+					Seq.length line_before > 1 /\
+					Seq.length line_before >= 1+ (fst (get_bytes_push 1 line_before))} ->
+				result_before : bool {result_before = true} -> 
+				Tot(st:stackBC (seq nat) {Stack.length st = Stack.length st_before + 1} * 
+				line: seq nat {Seq.length line = Seq.length line_before -1 - fst(get_bytes_push 1 line_before)} * result:bool)
+
+let op_push1 st_before line_before result_before = 
+	let bytes = get_bytes_push 1 line_before in 
+	let length = fst bytes in 
+	let line_new = snd bytes in 
+	let element = Seq.split line_new length in 
+	let stack_push1 = Stack.push st_before (fst element) in 
+	(stack_push1, snd element, result_before)
+
+val op_push2: st_before : stackBC (seq nat) {Stack.capacity st_before > 0} ->
+				line_before : seq nat {
+					Seq.length line_before > 0 /\ Seq.head line_before = 77 /\ 
+					Seq.length line_before > 2 /\
+					Seq.length line_before >= 2 + (fst (get_bytes_push 2 line_before))} ->
+				result_before : bool {result_before = true} -> 
+				Tot(st:stackBC (seq nat) {Stack.length st = Stack.length st_before + 1} * 
+				line: seq nat {Seq.length line = Seq.length line_before -2  - fst(get_bytes_push 2 line_before)} * result:bool)
+
+let op_push2 st_before line_before result_before = 
+	let bytes = get_bytes_push 2 line_before in 
+	let length = fst bytes in 
+	let line_new = snd bytes in 
+	let element = Seq.split line_new length in 
+	let stack_push1 = Stack.push st_before (fst element) in 
+	(stack_push1, snd element, result_before)
+
+val op_push4: st_before : stackBC (seq nat) {Stack.capacity st_before > 0} ->
+				line_before : seq nat {
+					Seq.length line_before > 0 /\ Seq.head line_before = 78 /\ 
+					Seq.length line_before > 4 /\
+					Seq.length line_before >= 4+ (fst (get_bytes_push 4 line_before))} ->
+				result_before : bool {result_before = true} -> 
+				Tot(st:stackBC (seq nat) {Stack.length st = Stack.length st_before + 1} * 
+				line: seq nat {Seq.length line = Seq.length line_before -4  - fst(get_bytes_push 4 line_before)} * result:bool)
+
+let op_push4 st_before line_before result_before = 
+	let bytes = get_bytes_push 4 line_before in 
+	let length = fst bytes in 
+	let line_new = snd bytes in 
+	let element = Seq.split line_new length in 
+	let stack_push1 = Stack.push st_before (fst element) in 
+	(stack_push1, snd element, result_before)
+
+val op_negate: st_before : stackBC(seq nat) {Stack.capacity st_before > 0} -> 
+			line_before: seq nat {Seq.length line_before > 0 /\ Seq.head line_before = 79} ->
+			result_before : bool {result_before = true} -> 
+			Tot(st: stackBC (seq nat) {Stack.length st = Stack.length st_before + 1} *
+			line: seq nat {Seq.length line = Seq.length line_before -1} * result : bool )
+
+let op_negate st_before line_before result_before = 
+	let element = Seq.create 1 255 in
+	let stack_push1 = Stack.push  st_before element in 
+	let line = Seq.tail line_before in 
+	(stack_push1, line, result_before)
+
+val op_true : st_before : stackBC(seq nat) {Stack.capacity st_before > 0} -> 
+			line_before: seq nat {Seq.length line_before > 0 /\ Seq.head line_before = 81} ->
+			result_before : bool {result_before = true} -> 
+			Tot(st: stackBC (seq nat) {Stack.length st = Stack.length st_before + 1} *
+			line: seq nat {Seq.length line = Seq.length line_before -1} * result : bool )
+
+let op_true st_before line_before result_before = 
+	let element = Seq.create 1 1 in
+	let stack_push1 = Stack.push  st_before element in 
+	let line = Seq.tail line_before in 
+	(stack_push1, line, result_before)
+
+val op_2_16: st_before : stackBC(seq nat) {Stack.capacity st_before > 0} -> 
+			line_before: seq nat {Seq.length line_before > 0 /\ (Seq.head line_before > 81 /\ Seq.head  line_before < 97)} ->
+			result_before : bool {result_before = true} -> 
+			Tot(st: stackBC (seq nat) {Stack.length st = Stack.length st_before + 1} *
+			line: seq nat {Seq.length line = Seq.length line_before -1} * result : bool )
+
+(* 82 -> 2*)
+let op_2_16 st_before line_before result_before = 
+	let header = Seq.head line_before in 
+	let element =Seq.create 1 (header - 80) in 
+	let stack_push1 = Stack.push st_before element in 
+	let line = Seq.tail line_before in 
+	(stack_push1, line, result_before)
+
+val op_nop : st_before: stackBC(seq nat) -> 	
+			line_before : seq nat {Seq.length line_before > 0  /\ Seq. head line_before = 97} -> 
+			result_before : bool {result_before = true} -> 
+			Tot(st: stackBC (seq nat) {Stack.equal st_before st} *
+			line: seq nat {Seq.length line = Seq.length line_before -1} * result : bool	
+		)
+let op_nop st_before line_before result_before = 
+	let line = Seq.tail line_before in 
+	(st_before, line, result_before)
+
+val op_if : st_before : stackBC (seq nat){Stack.length st_before > 0} -> 
+			line_before : seq nat {Seq.length line_before  > 0 /\ (Seq.head line_before = 99 /\ (Seq.mem 104 line_before))} ->
+			result_before : bool {result_before = true} ->
+			Tot(st: stackBC (seq nat){Stack.length st = Stack.length st_before - 1} * line: seq nat * result : bool * if_flag: bool )
+
+
+(* if yes -> return command knowing that it was if *)
+(*  if not -> if there is else -> return to else otherwise to endif*)
+(* we need the information about if only if we came from the statement true *)
+let op_if st_before line_before result_before = 
+	let pop_el = Stack.pop st_before in 
+	let result_execution = fst pop_el in 
+	let stack_pop = snd pop_el in 
+	if Seq.eq result_execution (Seq.create 1 255) then
+		let line = Seq.tail line_before in (stack_pop, line, result_before, true)
+	else if 
+			(Seq.mem 103 line_before && 
+				((search line_before 103 ) > (search line_before 104 ))) then 
+					let index = search line_before 103 in 
+					let line = Seq.split line_before index in 
+					(stack_pop, snd line, result_before, false)
+	else 
+		let index = search  line_before 104  in 
+		let line = Seq.split line_before index in 
+				(stack_pop, snd line, result_before, false )
+
+val op_else: st_before : stackBC(seq nat) -> 
+			line_before : seq nat {Seq.length line_before  > 0 /\ Seq.head line_before = 103 /\ Seq.mem 104 line_before} -> 
+			result_before : bool {result_before = true} -> 
+			if_flag : bool {if_flag : true} -> 
+			Tot(st: stackBC (seq nat) * 
+			line: seq nat {Seq.length line = Seq.length line_before -1} * result : bool	)
+
+let op_else st_before line_before result_before if_flag = 
+			let line = Seq.tail line_before in 
+			(st_before, line, result_before) 
