SeqExtension.fst
@@ -1,0 +1,23 @@
+module SeqExtension
+
+open FStar.Seq
+open FStar.Option
+
+module Seq = FStar.Seq
+
+
+val _search: #a: eqtype -> s: seq a {Seq.length s > 0} -> element: a {Seq.mem element s}->  i: nat {i < Seq.length s} -> 
+			Tot(r: nat{r < Seq.length s})
+			(decreases (Seq.length s - i))			
+
+let rec _search #a  s element i= 
+	if (i = Seq.length s -1) then i else
+	if Seq.index s i = element then i 
+	else 
+		_search #a s element  (i + 1)
+
+val search: #a : eqtype ->s: seq a{Seq.length s > 0} -> element: a {Seq.mem element s}->  
+			Tot(r: nat{r < Seq.length s})
+
+let search #a  s element = 
+	_search #a  s element 0			
